untype_lambda/chap6.v
@@ -3,27 +3,58 @@ Inductive term : Type :=
 | Abs : term -> term
 | App : term -> term -> term.
 
+Notation beta_ShiftNum := 0.
+
 Fixpoint shift (d c: nat) (t: term) : term :=
   match t with
   | Var k =>
-    if Nat.leb c k then Var (k + d) else Var k
+    if Nat.leb c k then
+      match d with
+      | beta_ShiftNum => Var (k - 1)
+      | _ => Var (k + d)
+      end
+    else Var k
   | Abs t1 => Abs (shift d (c + 1) t1)
   | App t1 t2 => App (shift d c t1) (shift d c t2)
   end.
 
+Definition up (n: nat) (t: term) : term := shift n 0 t.
 
-Compute ( shift 2 0 (Abs (Abs (App (Var 1) (App (Var 0) (Var 2) ))))).
-Compute ( shift 2 0 (Abs (App (Var 0) (App (Var 1)(Abs (App (Var 0)(App (Var 1)(Var 2)))))))).
+Compute ( up 2 (Abs (Abs (App (Var 1) (App (Var 0) (Var 2) ))))). (* = Abs (Abs (App (Var 1) (App (Var 0) (Var 4)))) *)
+Compute ( up 2 (Abs (App (Var 0) (App (Var 1)(Abs (App (Var 0)(App (Var 1)(Var 2)))))))). (* = Abs (App (Var 0) (App (Var 3) (Abs (App (Var 0) (App (Var 1) (Var 4)))))) *)
 
 Fixpoint subst (j: nat) (s t: term) : term :=
   match t with
   | Var k =>
     if Nat.eqb j k then s else Var k
   | Abs t1 =>
-    Abs (subst (j + 1) (shift 1 0 s) t1)
+    Abs (subst (j + 1) (up 1 s) t1)
   | App t1 t2 =>
     App (subst j s t1) (subst j s t2)
   end.
 
-Compute (subst 0 (Var 1) (App (Var 0) (Abs(Abs (Var 2))))).
-Compute (subst 0 (App (Var 1) (Abs (Var 2))) (App (Var 0) (Abs (Var 1)))).
+Compute (subst 0 (Var 1) (App (Var 0) (Abs(Abs (Var 2))))).  (* = App (Var 1) (Abs (Abs (Var 3))) *)
+Compute (subst 0 (App (Var 1) (Abs (Var 2))) (App (Var 0) (Abs (Var 1)))). (* = App (App (Var 1) (Abs (Var 2))) (Abs (App (Var 2) (Abs (Var 3)))) *)
+
+Reserved Notation " t '-->' t' " (at level 40).
+
+Inductive value : term -> Prop :=
+  | v_abs : forall n,
+      value (Abs n).
+
+Notation "'[' x ':=' s ']' t" := (subst x s t) (at level 20).
+
+Inductive eval : term -> term -> Prop :=
+  | E_App1 : forall t1 t1' t2,
+         t1 --> t1' ->
+         App t1 t2 --> App t1' t2
+  | E_App2 : forall v1 t2 t2',
+         value v1 ->
+         t2 --> t2' ->
+         App v1 t2 --> App v1 t2'
+  | E_AppAbs : forall t1 v2,
+         value v2 ->
+         App (Abs t1) v2 -->
+             up beta_ShiftNum ([0 := up 1 (v2)] t1)
+
+  where " t '-->' t' " := (eval t t').
